Some models to reason about iterators on vecs

src/extract/ExtractBuiltinLean.ml
@@ -12,6 +12,9 @@ let lean_builtin_types =
            [ ("bytes", Some "bytes"); ("isValidUTF8", Some "isValidUTF8") ]);
     (* file: "Aeneas/Std/Vec.lean", line: 18 *)
     mk_type "alloc::vec::Vec" "alloc.vec.Vec";
+    (* file: "Aeneas/Std/Vec.lean", line: 241 *)
+    mk_type "alloc::vec::into_iter::IntoIter" "alloc.vec.into_iter.IntoIter"
+      ~keep_params:(Some [ true; false ]);
     (* file: "Aeneas/Std/Core/Ptr.lean", line: 78 *)
     mk_type "core::alloc::layout::Layout" "core.alloc.layout.Layout"
       ~kind:(KStruct [ ("size", Some "size"); ("align", Some "align") ]);
@@ -179,23 +182,34 @@ let lean_builtin_funs =
       "alloc.boxed.Box.deref_mut"
       ~keep_params:(Some [ true; false ])
       ~can_fail:false;
+    (* file: "Aeneas/Std/Vec.lean", line: 235 *)
+    mk_fun "alloc::slice::{[@T]}::into_vec" "alloc.slice.Slice.into_vec"
+      ~keep_params:(Some [ true; false ])
+      ~can_fail:false ~lift:false;
     (* file: "Aeneas/Std/Vec.lean", line: 223 *)
     mk_fun "alloc::slice::{[@T]}::to_vec" "alloc.slice.Slice.to_vec";
-    (* file: "Aeneas/Std/Vec.lean", line: 237 *)
+    (* file: "Aeneas/Std/Vec.lean", line: 259 *)
     mk_fun "alloc::vec::from_elem" "alloc.vec.from_elem";
-    (* file: "Aeneas/Std/Vec.lean", line: 368 *)
+    (* file: "Aeneas/Std/Vec.lean", line: 244 *)
+    mk_fun
+      "alloc::vec::into_iter::{core::iter::traits::iterator::Iterator<alloc::vec::into_iter::IntoIter<@T, \
+       @A>, @T>}::next"
+      "alloc.vec.into_iter.IteratorIntoIter.next"
+      ~keep_params:(Some [ true; false ])
+      ~can_fail:false;
+    (* file: "Aeneas/Std/Vec.lean", line: 403 *)
     mk_fun
       "alloc::vec::partial_eq::{core::cmp::PartialEq<alloc::vec::Vec<@T>, \
        alloc::vec::Vec<@U>>}::eq"
       "alloc.vec.partial_eq.PartialEqVec.eq"
       ~keep_params:(Some [ true; true; false; false ]);
-    (* file: "Aeneas/Std/Vec.lean", line: 378 *)
+    (* file: "Aeneas/Std/Vec.lean", line: 413 *)
     mk_fun
       "alloc::vec::partial_eq::{core::cmp::PartialEq<alloc::vec::Vec<@T>, \
        alloc::vec::Vec<@U>>}::ne"
       "alloc.vec.partial_eq.PartialEqVec.ne"
       ~keep_params:(Some [ true; true; false; false ]);
-    (* file: "Aeneas/Std/Vec.lean", line: 257 *)
+    (* file: "Aeneas/Std/Vec.lean", line: 279 *)
     mk_fun "alloc::vec::{alloc::vec::Vec<@T>}::extend_from_slice"
       "alloc.vec.Vec.extend_from_slice"
       ~keep_params:(Some [ true; false ]);
@@ -212,29 +226,40 @@ let lean_builtin_funs =
     (* file: "Aeneas/Std/Vec.lean", line: 100 *)
     mk_fun "alloc::vec::{alloc::vec::Vec<@T>}::push" "alloc.vec.Vec.push"
       ~keep_params:(Some [ true; false ]);
-    (* file: "Aeneas/Std/Vec.lean", line: 291 *)
+    (* file: "Aeneas/Std/Vec.lean", line: 313 *)
     mk_fun "alloc::vec::{alloc::vec::Vec<@T>}::resize" "alloc.vec.Vec.resize"
       ~keep_params:(Some [ true; false ]);
-    (* file: "Aeneas/Std/Vec.lean", line: 254 *)
+    (* file: "Aeneas/Std/Vec.lean", line: 276 *)
     mk_fun "alloc::vec::{alloc::vec::Vec<@T>}::with_capacity"
       "alloc.vec.Vec.with_capacity" ~can_fail:false ~lift:false;
-    (* file: "Aeneas/Std/Vec.lean", line: 355 *)
+    (* file: "Aeneas/Std/Vec.lean", line: 390 *)
     mk_fun "alloc::vec::{core::clone::Clone<alloc::vec::Vec<@T>>}::clone"
       "alloc.vec.CloneVec.clone"
       ~keep_params:(Some [ true; false ])
       ~keep_trait_clauses:(Some [ true; false ]);
-    (* file: "Aeneas/Std/Vec.lean", line: 318 *)
+    (* file: "Aeneas/Std/Vec.lean", line: 353 *)
     mk_fun
       "alloc::vec::{core::convert::From<Box<[@T]>, alloc::vec::Vec<@T>>}::from"
       "alloc.vec.FromBoxSliceVec.from"
       ~keep_params:(Some [ true; false ]);
-    (* file: "Aeneas/Std/Vec.lean", line: 268 *)
+    (* file: "Aeneas/Std/Vec.lean", line: 339 *)
+    mk_fun
+      "alloc::vec::{core::convert::From<alloc::vec::Vec<@T>, [@T; @N]>}::from"
+      "alloc.vec.FromVecArray.from" ~can_fail:false;
+    (* file: "Aeneas/Std/Vec.lean", line: 253 *)
+    mk_fun
+      "alloc::vec::{core::iter::traits::collect::IntoIterator<alloc::vec::Vec<@T>, \
+       @T, alloc::vec::into_iter::IntoIter<@T, @A>>}::into_iter"
+      "alloc.vec.IntoIteratorVec.into_iter"
+      ~keep_params:(Some [ true; false ])
+      ~can_fail:false ~lift:false;
+    (* file: "Aeneas/Std/Vec.lean", line: 290 *)
     mk_fun
       "alloc::vec::{core::ops::deref::Deref<alloc::vec::Vec<@T>, [@T]>}::deref"
       "alloc.vec.Vec.deref"
       ~keep_params:(Some [ true; false ])
       ~can_fail:false ~lift:false;
-    (* file: "Aeneas/Std/Vec.lean", line: 278 *)
+    (* file: "Aeneas/Std/Vec.lean", line: 300 *)
     mk_fun
       "alloc::vec::{core::ops::deref::DerefMut<alloc::vec::Vec<@T>, \
        [@T]>}::deref_mut"
@@ -667,11 +692,11 @@ let lean_builtin_trait_decls =
     (* file: "Aeneas/Std/Core/Hash.lean", line: 6 *)
     mk_trait_decl "core::hash::Hasher" "core.hash.Hasher"
       ~methods:[ ("finish", "finish"); ("write", "write") ];
-    (* file: "Aeneas/Std/Core/Iter.lean", line: 21 *)
+    (* file: "Aeneas/Std/Core/Iter.lean", line: 22 *)
     mk_trait_decl "core::iter::adapters::zip::TrustedRandomAccessNoCoerce"
       "core.iter.adapters.zip.TrustedRandomAccessNoCoerce"
       ~consts:[ ("MAY_HAVE_SIDE_EFFECT", "MAY_HAVE_SIDE_EFFECT") ];
-    (* file: "Aeneas/Std/Core/Iter.lean", line: 10 *)
+    (* file: "Aeneas/Std/Core/Iter.lean", line: 11 *)
     mk_trait_decl "core::iter::range::Step" "core.iter.range.Step"
       ~parent_clauses:[ "cloneInst"; "partialOrdInst" ]
       ~methods:
@@ -708,7 +733,7 @@ let lean_builtin_trait_decls =
     mk_trait_decl "core::iter::traits::exact_size::ExactSizeIterator"
       "core.iter.traits.exact_size.ExactSizeIterator"
       ~parent_clauses:[ "iteratorInst" ];
-    (* file: "Aeneas/Std/Core/Iter.lean", line: 27 *)
+    (* file: "Aeneas/Std/Core/Iter.lean", line: 28 *)
     mk_trait_decl "core::iter::traits::iterator::Iterator"
       "core.iter.traits.iterator.Iterator"
       ~methods:[ ("next", "next") ];
@@ -799,7 +824,7 @@ let lean_builtin_trait_impls =
     (* file: "Aeneas/Std/Core/Core.lean", line: 33 *)
     mk_trait_impl "core::clone::Clone<alloc::alloc::Global>"
       "core.core.clone.CloneGlobal";
-    (* file: "Aeneas/Std/Vec.lean", line: 361 *)
+    (* file: "Aeneas/Std/Vec.lean", line: 396 *)
     mk_trait_impl "core::clone::Clone<alloc::vec::Vec<@T>>"
       "core.clone.CloneallocvecVec"
       ~keep_params:(Some [ true; false ])
@@ -815,7 +840,7 @@ let lean_builtin_trait_impls =
     mk_trait_impl "core::cmp::PartialEq<Box<@T>, Box<@T>>"
       "core.cmp.PartialEqBox"
       ~keep_params:(Some [ true; false ]);
-    (* file: "Aeneas/Std/Vec.lean", line: 389 *)
+    (* file: "Aeneas/Std/Vec.lean", line: 424 *)
     mk_trait_impl
       "core::cmp::PartialEq<alloc::vec::Vec<@T>, alloc::vec::Vec<@U>>"
       "core.cmp.PartialEqVec"
@@ -826,10 +851,13 @@ let lean_builtin_trait_impls =
     mk_trait_impl "core::convert::AsMut<Box<@T>, @T>" "core.convert.AsMutBox";
     (* file: "Aeneas/Std/Core/Convert.lean", line: 29 *)
     mk_trait_impl "core::convert::From<@Self, @Self>" "core.convert.FromSame";
-    (* file: "Aeneas/Std/Vec.lean", line: 326 *)
+    (* file: "Aeneas/Std/Vec.lean", line: 361 *)
     mk_trait_impl "core::convert::From<Box<[@T]>, alloc::vec::Vec<@T>>"
       "core.convert.FromBoxSliceVec"
       ~keep_params:(Some [ true; false ]);
+    (* file: "Aeneas/Std/Vec.lean", line: 345 *)
+    mk_trait_impl "core::convert::From<alloc::vec::Vec<@T>, [@T; @N]>"
+      "core.convert.FromVecArray";
     (* file: "Aeneas/Std/Core/Convert.lean", line: 20 *)
     mk_trait_impl "core::convert::Into<@Self, @T>" "core.convert.IntoFrom";
     (* file: "Aeneas/Std/Array/ArraySlice.lean", line: 175 *)
@@ -856,6 +884,18 @@ let lean_builtin_trait_impls =
     (* file: "Aeneas/Std/Core/Iter.lean", line: 61 *)
     mk_trait_impl "core::iter::traits::collect::IntoIterator<@I, @Item, @I>"
       "core.iter.traits.collect.IntoIterator.Blanket";
+    (* file: "Aeneas/Std/Core/Iter.lean", line: 147 *)
+    mk_trait_impl
+      "core::iter::traits::collect::IntoIterator<alloc::vec::Vec<@T>, @T, \
+       alloc::vec::into_iter::IntoIter<@T, @A>>"
+      "core.iter.traits.collect.IntoIteratorVec"
+      ~keep_params:(Some [ true; false ]);
+    (* file: "Aeneas/Std/Core/Iter.lean", line: 139 *)
+    mk_trait_impl
+      "core::iter::traits::iterator::Iterator<alloc::vec::into_iter::IntoIter<@T, \
+       @A>, @T>"
+      "core.iter.traits.iterator.IteratorIntoIter"
+      ~keep_params:(Some [ true; false ]);
     (* file: "Aeneas/Std/Core/Iter.lean", line: 131 *)
     mk_trait_impl
       "core::iter::traits::iterator::Iterator<core::ops::range::Range<@A>, @A>"
@@ -865,14 +905,14 @@ let lean_builtin_trait_impls =
     (* file: "Aeneas/Std/Core/Ops.lean", line: 29 *)
     mk_trait_impl "core::ops::deref::Deref<Box<@T>, @T>"
       "core.ops.deref.DerefBoxInst";
-    (* file: "Aeneas/Std/Vec.lean", line: 273 *)
+    (* file: "Aeneas/Std/Vec.lean", line: 295 *)
     mk_trait_impl "core::ops::deref::Deref<alloc::vec::Vec<@T>, [@T]>"
       "core.ops.deref.DerefVec"
       ~keep_params:(Some [ true; false ]);
     (* file: "Aeneas/Std/Core/Ops.lean", line: 36 *)
     mk_trait_impl "core::ops::deref::DerefMut<Box<@T>, @T>"
       "core.ops.deref.DerefMutBoxInst";
-    (* file: "Aeneas/Std/Vec.lean", line: 284 *)
+    (* file: "Aeneas/Std/Vec.lean", line: 306 *)
     mk_trait_impl "core::ops::deref::DerefMut<alloc::vec::Vec<@T>, [@T]>"
       "core.ops.deref.DerefMutVec"
       ~keep_params:(Some [ true; false ]);
